Refactored a lot of files; added definition of base_of; finished circuit theorem

src/matroid.lean
@@ -3,21 +3,23 @@ import tactic
 import finset
 
 -- TODO: 
--- matroid constructions: subtype, contract, direct sum, map
+-- matroid constructions: subtype, contraction, direct sum, map
+-- dual matroid, matroid isomorphism
 -- base theorem, base construction
 -- circuit theorem, circuit construction
 -- rank theorem, rank construction
 -- closure theorem, closure construction
 -- examples
 
-structure matroid (X : Type*) [fintype X] [decidable_eq X] :=
-  (ind : set (finset X))
+structure matroid (α : Type*) [fintype α] [decidable_eq α] :=
+  (ind : set (finset α))
+  [ind_dec : decidable_pred ind]
   (ind_empty : ind ∅)
   (ind_subset : ∀ (A B), A ⊆ B → ind B → ind A)
-  (ind_exchange : ∀ (A B : finset X), A ∈ ind → B ∈ ind → A.card < B.card →
+  (ind_exchange : ∀ (A B : finset α), ind A → ind B → A.card < B.card →
     (∃ (c ∈ B), (c ∉ A) ∧ ind (insert c A)))
 
-variables {X : Type*} [fintype X] [decidable_eq X] {m : matroid X}
+variables {α : Type*} [fintype α] [decidable_eq α] {m : matroid α} {A X : finset α}
 
 open finset
 
@@ -27,14 +29,23 @@ namespace matroid
 
 @[simp] lemma ind_subset_def : ∀ (A B), A ⊆ B → m.ind B → m.ind A := m.ind_subset
 
-def base (m : matroid X) (A : finset X) := m.ind A ∧ ∀ x ∉ A, ¬m.ind (insert x A)
+@[simp] lemma dep_superset {A B} : A ⊆ B → ¬m.ind A → ¬m.ind B := λ h hA hB, hA (m.ind_subset _ _ h hB)
 
-@[simp] lemma base_ind {A : finset X} : m.base A → m.ind A := λ x, x.1
+def base (m : matroid α) (A : finset α) := m.ind A ∧ ∀ x ∉ A, ¬m.ind (insert x A)
 
-def circuit (m : matroid X) (C : finset X) := ¬ m.ind C ∧ ∀ x ∈ C, m.ind (C.erase x)
+def base_of (m : matroid α) (A B : finset α) := B ⊆ A ∧ m.ind B ∧ ∀ (x ∉ B), (x ∈ A) → ¬m.ind (insert x B) 
 
-@[simp] lemma circuit_not_ind {C : finset X} : m.circuit C → ¬ m.ind C := λ x, x.1
+@[simp] lemma base_ind : m.base A → m.ind A := λ h, h.1
 
+@[simp] lemma base_of_ind : m.base_of X A → m.ind A := λ h, h.2.1
 
+@[simp] lemma base_of_subset : m.base_of X A → A ⊆ X := λ h, h.1
+
+@[simp] lemma base_of_univ_iff_base {A : finset α} : m.base_of univ A ↔ m.base A :=
+  ⟨λ ⟨_, h_ind, h_ins⟩, ⟨h_ind, λ x hx, h_ins x hx (mem_univ x)⟩, λ ⟨h_ind, h_ins⟩, ⟨subset_univ A, h_ind, λ x hx _, h_ins x hx⟩⟩
+
+def circuit (m : matroid α) (A : finset α) := ¬ m.ind A ∧ ∀ x ∈ A, m.ind (A.erase x)
+
+@[simp] lemma circuit_dep : m.circuit A → ¬ m.ind A := λ x, x.1
 
 end matroid
