src/base.lean
@@ -2,49 +2,24 @@ import data.fintype.basic
 import tactic
 import matroid
 import finset
+import base_of
 
-variables {X : Type*} [fintype X] [decidable_eq X] {m : matroid X}
+variables {α : Type*} [fintype α] [decidable_eq α] {m : matroid α} {A B: finset α}
 
 open finset
 
 namespace matroid
 
-lemma base_eq_card {A B : finset X} (hA : m.base A) (hB : m.base B) : A.card = B.card := 
-begin
-  by_contradiction,
-  wlog : A.card ≤ B.card := le_total A.card B.card using [A B, B A],
-  replace h := nat.lt_of_le_and_ne case h,
-  rcases m.ind_exchange _ _ (base_ind hA) (base_ind hB) h with ⟨w, wB, wA, winsert⟩,
-  exact hA.2 w wA winsert,
+lemma base_eq_card (hA : m.base A) (hB : m.base B) : A.card = B.card := 
+  by {rw [←base_of_univ_iff_base] at *, exact base_of_eq_card hA hB} 
+
+lemma ind_subset_base : m.ind A → ∃ B, A ⊆ B ∧ m.base B := λ hA, begin
+  obtain ⟨B, hAB, h_base⟩ := ind_subset_base_of (subset_univ A) hA,
+  rw base_of_univ_iff_base at h_base,
+  use [B, hAB, h_base],
 end
 
-lemma ind_subset_base {A} : m.ind A → ∃ B, A ⊆ B ∧ m.base B :=
-begin
-  intro Aind,
-  by_contradiction,
-  push_neg at h,
-  suffices ind_unbounded : ∀ k ≥ A.card, ∃ B, A ⊆ B ∧ (m.ind B) ∧ B.card = k, {
-    rcases ind_unbounded (fintype.card X + 1) _ with ⟨B, h_suibset, Bind, Bcard⟩,
-    have Bcard_le := card_le_univ B,
-    linarith,
-    have Acard_le := card_le_univ A,
-    linarith,
-  },
-  apply nat.le_induction, {
-    use [A, subset.refl A, Aind, rfl],
-  }, {
-    rintro n Acard ⟨B, h_subset, Bind, Bcard⟩,
-    specialize h B h_subset,
-    rw base at h,
-    push_neg at h,
-    rcases h Bind with ⟨x, xB, x_insert⟩,
-    use [insert x B],
-    rw ← Bcard,
-    use [subset.trans h_subset (subset_insert _ _), x_insert, card_insert_of_not_mem xB],
-  }
-end
-
-theorem base_exists : ∃ A, m.base A :=
+theorem exists_base : ∃ A, m.base A := 
 begin
   obtain ⟨B, _, Bbase⟩ := ind_subset_base m.ind_empty,
   exact ⟨B, Bbase⟩,
@@ -53,7 +28,7 @@ end
 theorem base_not_subset {A B} : m.base A → m.base B → A ⊆ B → A = B :=
 begin
   rintro Abase Bbase h_subset,
-  exact finset.eq_of_subset_card_eq_card h_subset (base_eq_card Abase Bbase),
+  exact eq_of_subset_of_card_le h_subset (ge_of_eq $ base_eq_card Abase Bbase),
 end
 
 lemma ind_and_card_eq_card_base_iff_base {A B} (Abase : m.base A) : (m.ind B ∧ A.card = B.card) ↔ m.base B :=
