src/base_of.lean
@@ -1,0 +1,62 @@
+import data.fintype.basic
+import tactic
+import matroid
+import finset
+
+variables {α : Type*} [fintype α] [decidable_eq α] {m : matroid α} {A B X: finset α}
+
+open finset
+
+namespace matroid
+
+lemma base_of_eq_card (hA : m.base_of X A) (hB : m.base_of X B) : A.card = B.card := 
+begin
+  by_contradiction,
+  wlog : A.card ≤ B.card := le_total A.card B.card using [A B, B A],
+  replace h := nat.lt_of_le_and_ne case h,
+  obtain ⟨w, wB, wA, winsert⟩ := m.ind_exchange _ _ (base_of_ind hA) (base_of_ind hB) h,
+  refine hA.2.2 w wA (base_of_subset hB wB) winsert,
+end
+
+lemma ind_subset_base_of : A ⊆ X → m.ind A → ∃ B, A ⊆ B ∧ m.base_of X B :=
+begin
+  intros hAX hA,
+  by_contradiction,
+  push_neg at h,
+  suffices ind_unbounded : ∀ k ≥ A.card, ∃ B, A ⊆ B ∧ B ⊆ X ∧ m.ind B ∧ B.card = k, {
+    rcases ind_unbounded (X.card + 1) _ with ⟨B, hAB, hBX, Bind, Bcard⟩,    
+    replace hBX := card_le_of_subset hBX,
+    linarith, 
+    replace hAX := card_le_of_subset hAX,
+    linarith,
+  },
+  apply nat.le_induction, {
+    use [A, subset.refl A, hAX, hA],
+  }, {
+    rintro n Acard ⟨B, hAB, hBX, Bind, rfl⟩,
+    specialize h B hAB,
+    rw base_of at h,
+    push_neg at h,
+    rcases h hBX Bind with ⟨w, wB, wX, w_insert⟩,
+    use [insert w B],
+    use [subset.trans hAB (subset_insert _ _)],
+    use [insert_subset.2 ⟨wX, hBX⟩],
+    use [w_insert, card_insert_of_not_mem wB],
+  }
+end
+
+theorem exists_base_of (m : matroid α) (X : finset α): ∃ A, m.base_of X A :=
+begin
+  obtain ⟨B, _, Bbase⟩ := ind_subset_base_of (empty_subset X) m.ind_empty,
+  exact ⟨B, Bbase⟩,
+end
+
+lemma ind_card_le_base_of_card : (A ⊆ X) → m.ind A → m.base_of X B → A.card ≤ B.card :=
+begin
+  intros hAX Aind Bbase,
+  obtain ⟨T, hAT, Tbase⟩ := ind_subset_base_of hAX Aind,
+  rw base_of_eq_card Bbase Tbase,
+  exact card_le_of_subset hAT,
+end
+
+end matroid
