src/circuit.lean
@@ -1,15 +1,17 @@
-import data.fintype.basic
+import data.nat.basic
+import data.finset.basic
 import tactic
 import matroid
 import finset
+import base_of
 
-variables {X : Type*} [fintype X] [decidable_eq X] {m : matroid X}
+variables {α : Type*} [fintype α] [decidable_eq α] {m : matroid α} {A B : finset α}
 
 open finset
 
 namespace matroid
 
-lemma circuit_sdiff {A B} : m.circuit A → B ⊆ A → B ≠ ∅ → m.ind (A \ B) :=
+lemma circuit_sdiff  : m.circuit A → B ⊆ A → B ≠ ∅ → m.ind (A \ B) :=
 begin
   rintro ⟨Anind, Aerase⟩ Bsubset Bnonempty, 
   rw ← nonempty_iff_ne_empty at Bnonempty,
@@ -19,7 +21,7 @@ begin
   exact sdiff_subset_erase_of_mem xB,
 end 
 
-lemma circuit_subset {A B} : m.circuit A → B ⊂ A → m.ind B :=
+lemma circuit_ssubset : m.circuit A → B ⊂ A → m.ind B :=
 begin 
   rintro ⟨Anind, Aerase⟩ Bsubset,
   rw ssubset_iff at Bsubset,
@@ -29,6 +31,94 @@ begin
   apply m.ind_subset _ (A.erase x) _ (Aerase x xA),
   rw ← erase_eq_of_not_mem xB,
   exact erase_subset_erase x h_subset,
-end 
+end
+
+lemma ind_iff_not_contains_circuit (A) : m.ind A ↔ ∀ C, m.circuit C → ¬ C ⊆ A :=
+begin
+  split, {
+    intros Aind C Ccirc hCA,
+    refine dep_superset hCA (Ccirc.1) Aind,
+  }, {
+    intros h,
+    by_contradiction Aind,
+    suffices subsets_dep : ∀ k ≤ A.card, ∃ B ⊆ A, B.card = k ∧ ¬ m.ind B, {
+      obtain ⟨B, Bsub, Bcard, Bdep⟩ := subsets_dep 0 (zero_le _),
+      rw [card_eq_zero] at Bcard,
+      subst Bcard,
+      exact Bdep m.ind_empty,
+    },
+    intros k k_le_card,
+    refine nat.decreasing_induction (λ n, _) k_le_card _, {
+      rintro ⟨B, hBA, Bcard, Bdep⟩,
+      specialize h B,
+      rw imp_not_comm at h,
+      specialize h hBA,
+      rw circuit at h,
+      push_neg at h,
+      obtain ⟨x, xAB, h_dep_erase⟩ := h Bdep,
+      refine ⟨B.erase x, subset.trans (erase_subset _ _) hBA, _, h_dep_erase⟩,
+      rw ← card_erase_of_mem' xAB at Bcard,
+      exact nat.succ_inj'.1 Bcard,
+    }, {
+      use [A, subset.refl _, rfl],
+    }
+  }
+end
+
+lemma dep_iff_contains_circuit (A) : ¬ m.ind A ↔ ∃ C, m.circuit C ∧ C ⊆ A :=
+begin
+  have h := not_congr (ind_iff_not_contains_circuit A),
+  push_neg at h,
+  exact h,
+end
+
+theorem empty_not_circuit : ¬ m.circuit ∅ := λ ⟨empty_dep, _⟩, empty_dep m.ind_empty
+
+theorem circuit_not_subset {A B} : m.circuit A → m.circuit B → A ⊆ B → A = B :=
+begin
+  rintro Acirc Bcirc h_subset,
+  cases eq_or_ssubset_of_subset h_subset,
+  { exact h, },
+  {
+    exfalso,
+    exact Acirc.1 (circuit_ssubset Bcirc h),
+  },
+end
+
+theorem circuit_common_element {x} (Acirc : m.circuit A) (Bcirc : m.circuit B): 
+  A ≠ B → x ∈ A → x ∈ B → ∃ C, m.circuit C ∧ C ⊆ ((A ∪ B).erase x) :=
+begin
+  intros A_neq_B xA xB, 
+  rw ← dep_iff_contains_circuit,
+  intro union_ind,
+  have inter_ind : m.ind (A ∩ B), from by {
+    rw ind_iff_not_contains_circuit,
+    intros C Ccirc Csub,
+    have hAC := circuit_not_subset Ccirc Acirc (subset.trans Csub (inter_subset_left _ _)),
+    have hBC := circuit_not_subset Ccirc Bcirc (subset.trans Csub (inter_subset_right _ _)),
+    exact A_neq_B (eq.trans hAC.symm hBC),
+  },
+  have tmp : A ∩ B ⊆ A ∪ B := subset.trans (inter_subset_left _ _) (subset_union_left _ _),
+  obtain ⟨X, hABX, hXbase_of⟩ := ind_subset_base_of tmp (inter_ind),
+  have tmp2 := ind_card_le_base_of_card (erase_subset _ _) union_ind hXbase_of,
+  
+  replace tmp2 := nat.add_le_add_right tmp2 1, 
+  rw [card_erase_of_mem' (mem_union_left _ xA)] at tmp2,
+  have tmp3 := card_le_of_subset hXbase_of.1,
+  cases eq_or_eq_succ_of_le_and_le_succ tmp3 tmp2, {
+    replace h := eq_of_subset_of_card_le (hXbase_of.1) (ge_of_eq h),
+    subst h,
+    refine (dep_iff_contains_circuit (A ∪ B)).2 _ hXbase_of.2.1,
+    use [A, Acirc, subset_union_left _ _],
+  }, {
+    cases very_important_lemma hABX hXbase_of.1 h.symm, {
+      refine (dep_iff_contains_circuit X).2 _ hXbase_of.2.1,
+      use [A, Acirc, h_1],
+    }, {
+      refine (dep_iff_contains_circuit X).2 _ hXbase_of.2.1,
+      use [B, Bcirc, h_1],      
+    }
+  }
+end
 
 end matroid
