src/finset.lean
@@ -14,36 +14,68 @@ begin
   exact card_ne_zero_of_mem h,
 end
 
-lemma eq_of_subset_card_eq_card {A B : finset X} : A ⊆ B → A.card = B.card → A = B :=
-begin
-  intros h_subset h_card,
-  induction B using finset.induction_on generalizing A, {
-    simpa only [card_empty, card_eq_zero] using h_card,
-  },
-  case h₂ : x B x_mem ih {
-    rw subset_insert_iff at h_subset,
-    rw card_insert_of_not_mem x_mem at h_card,
-    have t : x ∈ A, from by {
-      by_contradiction,
-      replace h_subset := card_le_of_subset h_subset,
-      rw [erase_eq_of_not_mem h, h_card] at h_subset,
-      simpa only [add_le_iff_nonpos_right, nonpos_iff_eq_zero] using h_subset,
-    },
-    rw [← card_erase_of_mem' t, add_left_inj] at h_card,
-    specialize ih h_subset h_card,
-    apply_fun insert x at ih,
-    rwa insert_erase t at ih,
-  },
-end
-
-example {A : finset X} {x} : A.erase x = A \ {x} := (sdiff_singleton_eq_erase x A).symm
-
 lemma sdiff_subset_erase_of_mem {A B : finset X} {x} : x ∈ B → A \ B ⊆ A.erase x :=
 begin
   intros xB,
   rw [← sdiff_singleton_eq_erase x A],
   apply sdiff_subset_sdiff (subset.refl _) _,
   rwa singleton_subset_iff,
+end
+
+lemma eq_or_ssubset_of_subset {A B : finset X} (h : A ⊆ B) : A = B ∨ A ⊂ B :=
+begin
+  rwa [← le_iff_subset, le_iff_eq_or_lt] at h,
+end
+
+lemma union_singleton {A : finset X} {x : X} : {x} ∪ A  = insert x A :=
+begin
+  exact (insert_eq x A).symm,
+end
+
+lemma card_succ_iff_erase_mem {A B : finset X} (h : A ⊆ B) :
+  B.card = A.card + 1 ↔ ∃ x ∈ B, A = B.erase x :=
+begin
+  split, {
+    intro h_card,
+    have hC : (B \ A).card = 1, from by {
+      rw [card_sdiff h],
+      exact nat.sub_eq_of_eq_add h_card,
+    },
+    obtain ⟨x, h_sing⟩ := card_eq_one.1 hC,
+    use x,
+    have hx : x ∈ B \ A, by simp only [h_sing, mem_singleton],
+    rw mem_sdiff at hx,
+    use hx.1,
+    rw [←sdiff_union_of_subset h, h_sing, ←insert_eq, erase_insert hx.2],
+  }, {
+    rintro ⟨x, xB, rfl⟩,
+    exact (card_erase_of_mem' xB).symm,
+  }
+end
+
+lemma very_important_lemma {A B S : finset X} : 
+  (A ∩ B) ⊆ S → S ⊆ (A ∪ B) → (A ∪ B).card = S.card + 1 → (A ⊆ S ∨ B ⊆ S) :=
+begin
+  intros ABS SAB Scard,
+  obtain ⟨x, xUnion, rfl⟩ := (card_succ_iff_erase_mem SAB).1 Scard,
+  rw mem_union at xUnion,
+  wlog xA : x ∈ A := xUnion using [A B, B A],
+  right,
+  have xInter : x ∉ A ∩ B := λ h, not_mem_erase _ _ (ABS h),
+  have xB : x ∉ B := λ h, xInter $ mem_inter_of_mem xA h,
+  nth_rewrite 0 ← (erase_eq_of_not_mem xB),
+  exact erase_subset_erase _ (subset_union_right _ _),
+end
+
+lemma eq_or_eq_succ_of_le_and_le_succ {x y : ℕ}: x ≤ y → y ≤ x + 1 → x = y ∨ x + 1 = y :=
+begin
+  intros hxy hyx1,
+  cases le_iff_lt_or_eq.1 hxy, {
+    right,
+    linarith,
+  }, {
+    left, exact h,
+  }
 end
 
 end finset
